\begin{align*}
E(R,t) &= \sum_{j=1}\lVert y_j - Rx_j - t \rVert_2^2
\end{align*}
We know that,from class,
\begin{align*}
\underset{R,t}{\operatorname{min}} E(R,t)&:\\
t^* &= \bar{Y} - R\bar{X} \\
R^* &= \underset{R}{\operatorname{min}}\lVert Y-RX \rVert_F^2\\
&=  \underset{R}{\operatorname{min}}\lVert Y \rVert_F^2 - 2\langle Y, RX \rangle + \lVert RX \rVert_F^2\\
&= \underset{R}{\operatorname{min}} -\langle Y,RX \rangle \\
&= \underset{R}{\operatorname{max}} \langle Y,RX \rangle \\
R^* &= \underset{R}{\operatorname{max}} \text{ trace}(Y^T RX) 
\end{align*}
We also know from class that $R$ is of the form:
\begin{align*}
R &=
\begin{pmatrix}
\cos\theta & -\sin\theta \\
\sin\theta & \cos\theta\\
\end{pmatrix}\\
R &= I\cos\theta + 
\begin{pmatrix}
0 & -1 \\ 1 & 0
\end{pmatrix}
\sin\theta \\
\therefore R^* &=
\begin{pmatrix}
\cos\theta^* & -\sin\theta^* \\
\sin\theta^* & \cos\theta^*\\
\end{pmatrix}
\end{align*}
Where, 
\begin{align*}
\theta^* &= \underset{\theta}{\operatorname{max}} \text{ trace}(Y^YRX)^T\\
&= \underset{\theta}{\operatorname{max}} \text{ trace}(X^T R^TY)\\
&= \underset{\theta}{\operatorname{max}} \text{ trace}(X^T(I\cos\theta + 
\begin{pmatrix}
0 & 1 \\ -1 & 0
\end{pmatrix}
\sin\theta)Y)\\
&= \underset{\theta}{\operatorname{max}} \text{ trace}(X^T Y\cos\theta) + \text{ trace}(X^T 
\begin{pmatrix}
0 & 1 \\ -1 & 0
\end{pmatrix}
Y\sin\theta)\\
0 &= \frac{\partial}{\partial\theta}
\begin{bmatrix}
\text{ trace}(X^T Y\cos\theta) + \text{ trace}(X^T 
\begin{pmatrix}
0 & 1 \\ -1 & 0
\end{pmatrix}
Y\sin\theta)
\end{bmatrix}\\
\text{ trace}(X^T Y)\sin\theta &= \text{ trace}(X^T 
\begin{pmatrix}
0 & 1 \\ -1 & 0
\end{pmatrix}
Y)\cos\theta \\
\end{align*}
We can now see that
\begin{align*}
\theta^* &= \arctan
\begin{pmatrix}
\frac{\text{ trace}(X^T
\begin{pmatrix}
0 & 1 \\ -1 & 0
\end{pmatrix}
Y)}{\text{ trace}(X^TY)}
\end{pmatrix} \\
\sin(\theta^*) &= \frac{\text{ trace}(X^T
\begin{pmatrix}
0 & 1 \\ -1 & 0
\end{pmatrix}
Y)}{\sqrt{\text{ trace}(X^TY)^2 + \text{ trace}(X^T
\begin{pmatrix}
0 & 1 \\ -1 & 0
\end{pmatrix}
Y)^2}} \\
\cos(\theta^*) &= \frac{\text{ trace}(X^TY)}{\sqrt{\text{ trace}(X^TY)^2 + \text{ trace}(X^T
\begin{pmatrix}
0 & 1 \\ -1 & 0
\end{pmatrix}
Y)^2}} \\
\end{align*}
$\therefore$ we can sub in $\sin(\theta^*)$ and $\cos(\theta^*)$ into $R$ and find that\\
\begin{align*}
R &= \frac{
\begin{pmatrix}
\text{ trace}(X^T Y) & -\text{ trace}(X^T \begin{pmatrix} 0 & 1 \\ -1 & 0 \end{pmatrix} Y) \\
\text{ trace}(X^T \begin{pmatrix} 0 & 1 \\ -1 & 0 \end{pmatrix} Y)  & \text{ trace}(X^T Y) \\
\end{pmatrix}}{\sqrt{\text{ trace}(X^TY)^2 + \text{ trace}(X^T \begin{pmatrix} 0 & 1 \\ -1 & 0 \end{pmatrix} Y)^2}}
\end{align*}
